moving norm related things from prims to pervasives

ulib/ml/prims.ml
@@ -154,27 +154,6 @@ let __proj__Cons__item__tl = List.tl
 
 let min = min
 
-type norm_step =
-    | Simpl
-    | Weak
-    | HNF
-    | Primops
-    | Delta
-    | Zeta
-    | Iota
-    | UnfoldOnly : string list -> norm_step
-    | UnfoldFully : string list -> norm_step
-
-let simplify : norm_step = Simpl
-let weak    : norm_step = Weak
-let hnf     : norm_step = HNF
-let primops : norm_step = Primops
-let delta   : norm_step = Delta
-let zeta    : norm_step = Zeta
-let iota    : norm_step = Iota
-let delta_only (s:string list) : norm_step = UnfoldOnly s
-let delta_fully (s:string list) : norm_step = UnfoldFully s
-
 type ('a, 'b) admit = unit
 
 let singleton x = x
