ulib/tactics_ml/FStar_Tactics_Builtins.ml
@@ -1,4 +1,5 @@
 open Prims
+open FStar_Pervasives_Native
 open FStar_Tactics_Result
 open FStar_Tactics_Types
 open FStar_Tactics_Effect
