ulib/FStar.Pervasives.Native.fst
@@ -69,3 +69,45 @@ type tuple8 'a 'b 'c 'd 'e 'f 'g 'h =
            -> _7:'g
            -> _8:'h
            -> tuple8 'a 'b 'c 'd 'e 'f 'g 'h
+
+
+(*********************************************************************************)
+(* Marking terms for normalization *)
+(*********************************************************************************)
+abstract let normalize_term (#a:Type) (x:a) : a = x
+abstract let normalize (a:Type0) :Type0 = a
+
+abstract
+noeq type norm_step =
+  | Simpl
+  | Weak
+  | HNF
+  | Primops
+  | Delta
+  | Zeta
+  | Iota
+  | UnfoldOnly:list string -> norm_step // each string is a fully qualified name like `A.M.f`
+  | UnfoldFully:list string -> norm_step // idem
+  | UnfoldAttr:#t:Type0 -> a:t -> norm_step
+
+// Helpers, so we don't expose the actual inductive
+abstract let simplify : norm_step = Simpl
+abstract let weak     : norm_step = Weak
+abstract let hnf      : norm_step = HNF
+abstract let primops  : norm_step = Primops
+abstract let delta    : norm_step = Delta
+abstract let zeta     : norm_step = Zeta
+abstract let iota     : norm_step = Iota
+abstract let delta_only (s:list string) : norm_step = UnfoldOnly s
+abstract let delta_fully (s:list string) : norm_step = UnfoldFully s
+abstract let delta_attr (#t:Type)(a:t) : norm_step = UnfoldAttr a
+
+// Normalization marker
+abstract let norm (s:list norm_step) (#a:Type) (x:a) : a = x
+
+abstract val assert_norm : p:Type -> Pure unit (requires (normalize p)) (ensures (fun _ -> p))
+let assert_norm p = ()
+
+let normalize_term_spec (#a: Type) (x: a) : Lemma (normalize_term #a x == x) = ()
+let normalize_spec (a: Type0) : Lemma (normalize a == a) = ()
+let norm_spec (s: list norm_step) (#a: Type) (x: a) : Lemma (norm s #a x == x) = ()
